Some IntoValTyped instances for primitive types

new/golang/theory/typing.v
@@ -7,8 +7,6 @@ From Ltac2 Require Import Ltac2.
 Set Default Proof Mode "Classic".
 From New.golang.defn Require Export typing mem.
 
-Section defs.
-
 Class IntoValProof (V : Type) `{IntoVal V} :=
   {
     typed_pointsto_def `{sem: ffi_semantics} `{!ffi_interp ffi} `{!heapGS Σ}
@@ -16,12 +14,14 @@ Class IntoValProof (V : Type) `{IntoVal V} :=
     #[global] to_val_inj :: Inj (=) (=) (to_val (V:=V));
     #[global] to_val_eqdec :: EqDecision V ;
   }.
-
-Notation typed_pointsto := typed_pointsto_def.
+Program Definition typed_pointsto := sealed @typed_pointsto_def.
+Definition typed_pointsto_unseal : typed_pointsto = _ := seal_eq _.
+Arguments typed_pointsto {_ _ _ _ _ _ _ _ _ _} (l dq v).
 Notation "l ↦ dq v" := (typed_pointsto l dq v%V)
                          (at level 20, dq custom dfrac at level 1,
                             format "l  ↦ dq  v") : bi_scope.
 
+Section defs.
 Context `{sem: ffi_semantics} `{!ffi_interp ffi} `{!heapGS Σ}.
 Context `{!NamedUnderlyingTypes}.
 Class IntoValTyped (V : Type) (t : go.type) `{!IntoVal V} `{!IntoValProof V} :=
@@ -36,142 +36,3 @@ Class IntoValTyped (V : Type) (t : go.type) `{!IntoVal V} `{!IntoValProof V} :=
 (* [ty] should not be an evar before doing typeclass search *)
 Global Hint Mode IntoValTyped - ! - - : typeclass_instances.
 End defs.
-
-Notation typed_pointsto := typed_pointsto_def.
-Notation "l ↦ dq v" := (typed_pointsto l dq v%V)
-                         (at level 20, dq custom dfrac at level 1,
-                            format "l  ↦ dq  v") : bi_scope.
-
-
-Section into_val_instances.
-Context `{sem: ffi_semantics} `{!ffi_interp ffi} `{!heapGS Σ}.
-
-Program Global Instance into_val_inj_loc : IntoValProof loc :=
-  {| typed_pointsto_def _ _ _ _ _ _ l dq v := heap_pointsto l dq #v |}.
-Next Obligation. rewrite to_val_unseal => ?? [=] //. Qed.
-
-(*
-Program Global Instance into_val_typed_loc t : IntoValTyped loc (go.PointerType t).
-Next Obligation. Admitted.
-Next Obligation. Admitted.
-
-Program Global Instance into_val_typed_w64 : IntoValTyped w64 uint64T :=
-{| default_val := W64 0 |}.
-Next Obligation. solve_has_go_type. Qed.
-Next Obligation. rewrite zero_val_eq //. Qed.
-Next Obligation. rewrite to_val_unseal => ?? [=] //. Qed.
-
-Program Global Instance into_val_typed_w32 : IntoValTyped w32 uint32T :=
-{| default_val := W32 0 |}.
-Next Obligation. solve_has_go_type. Qed.
-Next Obligation. rewrite zero_val_eq //. Qed.
-Next Obligation. rewrite to_val_unseal => ?? [=] //. Qed.
-
-Program Global Instance into_val_typed_w16 : IntoValTyped w16 uint16T :=
-{| default_val := W16 0 |}.
-Next Obligation. solve_has_go_type. Qed.
-Next Obligation. rewrite zero_val_eq //. Qed.
-Next Obligation. rewrite to_val_unseal => ?? [=] //. Qed.
-
-Program Global Instance into_val_typed_w8 : IntoValTyped w8 uint8T :=
-{| default_val := W8 0 |}.
-Next Obligation. solve_has_go_type. Qed.
-Next Obligation. rewrite zero_val_eq //. Qed.
-Next Obligation. rewrite to_val_unseal => ?? [=] //. Qed.
-
-Program Global Instance into_val_typed_bool : IntoValTyped bool boolT :=
-{| default_val := false |}.
-Next Obligation. solve_has_go_type. Qed.
-Next Obligation. rewrite zero_val_eq //. Qed.
-Next Obligation. rewrite to_val_unseal => ?? [=] //. Qed.
-
-Program Global Instance into_val_typed_string : IntoValTyped go_string stringT :=
-{| default_val := ""%go |}.
-Next Obligation. solve_has_go_type. Qed.
-Next Obligation. rewrite zero_val_eq //. Qed.
-Next Obligation. rewrite to_val_unseal => ?? [=] //. Qed.
-
-Program Global Instance into_val_typed_slice : IntoValTyped slice.t sliceT :=
-{| default_val := slice.nil |}.
-Next Obligation. solve_has_go_type. Qed.
-Next Obligation. rewrite zero_val_eq //. Qed.
-Next Obligation. rewrite to_val_unseal. move => [???][???] [=].
-                 repeat intros [=->%to_val_inj]. done.
-Qed.
-
-(* Using [vec] here because the [to_val] must be a total function that always
-   meets [has_go_type]. An alternative could be a sigma type. *)
-Program Global Instance into_val_typed_array `{!IntoVal V} `{!IntoValTyped V t} n :
-  IntoValTyped (vec V n) (arrayT n t) :=
-{| default_val := vreplicate n (default_val _) |}.
-Next Obligation.
-  rewrite to_val_unseal /=.
-  solve_has_go_type.
-  induction v as [|].
-  - apply (has_go_type_array 0 t []); done.
-  - simpl in *.
-    inversion IHv. subst.
-    pose proof (has_go_type_array (S (length a)) t (#h::a) ltac:(done)) as Ht.
-    simpl in Ht. apply Ht. intros ? [|].
-    + subst. apply to_val_has_go_type.
-    + apply Helems. done.
-Qed.
-Next Obligation.
-  intros.
-  rewrite to_val_unseal zero_val_eq /=.
-  rewrite -zero_val_unseal -default_val_eq_zero_val.
-  induction n; first done. simpl. f_equal. apply IHn.
-Qed.
-Final Obligation.
-rewrite to_val_unseal.
-intros. intros ?? Heq.
-simpl in Heq.
-induction x.
-{ rewrite (VectorSpec.nil_spec y) //. }
-destruct y using vec_S_inv.
-simpl in *.
-injection Heq as Heq1 Heq.
-apply to_val_inj in Heq1. subst.
-f_equal. by apply IHx.
-Qed.
-
-Program Global Instance into_val_typed_func : IntoValTyped func.t funcT :=
-{| default_val := func.nil |}.
-Next Obligation. solve_has_go_type. Qed.
-Next Obligation. rewrite zero_val_eq //. Qed.
-Next Obligation. rewrite to_val_unseal => [[???] [???]] /= [=] //. naive_solver.
-Qed.
-Final Obligation. solve_decision. Qed.
-
-Program Global Instance into_val_typed_interface : IntoValTyped interface.t interfaceT :=
-{| default_val := interface.nil |}.
-Next Obligation. solve_has_go_type. Qed.
-Next Obligation. rewrite zero_val_eq //. Qed.
-Next Obligation.
-  rewrite to_val_unseal => [x y] Heq.
-  destruct x as [|], y as [|].
-  {
-    simpl in *.
-    injection Heq as Heq1 Heq2.
-    apply to_val_inj in Heq1. subst. done.
-  }
-  all: first [discriminate | reflexivity].
-Qed.
-Final Obligation.
-  solve_decision.
-Qed.
-
-Program Global Instance into_val_typed_unit : IntoValTyped unit (structT []) :=
-{| default_val := tt |}.
-Next Obligation.
-  intros [].
-  replace (#()) with (struct.val_aux (structT []) []).
-  2:{ rewrite struct.val_aux_unseal //. }
-  by constructor.
-Qed.
-Next Obligation. rewrite zero_val_eq /= struct.val_aux_unseal //. Qed.
-Final Obligation.
-  intros ???. destruct x, y. done.
-Qed. *)
-
-End into_val_instances.
